reformulate group predicates and add more definitions and problems to real analysis

math/Artin2_1.dfy
@@ -36,26 +36,49 @@ module Artin {
     //!A signifies type invariance
     datatype Group<!A> = Group(elements: set<A>, identity: A, compose: (A,A) -> A, inverse: (A) -> A)
 
-    predicate isIdentity<A>(g: Group<A>) {
-        forall a :: a in g.elements ==> g.compose(a,g.identity) == a && g.compose(g.identity, a) == a
+    ghost predicate isIdentity<A(!new)>(g: Group<A>) {
+        forall a :: inGroup(g,a) ==> g.compose(a,g.identity) == a && g.compose(g.identity, a) == a
     }
 
-    predicate closedComposition<A>(g: Group<A>) {
-        forall x,y :: x in g.elements && y in g.elements ==> g.compose(x,y) in g.elements
+    lemma GroupIdentity<A>(g: Group<A>, a: A) 
+        requires inGroup(g, a)
+        ensures g.compose(a,g.identity) == a && g.compose(g.identity, a) == a
+    
+
+    ghost predicate closedComposition<A(!new)>(g: Group<A>) {
+        // forall x,y :: x in g.elements && y in g.elements ==> g.compose(x,y) in g.elements
+        forall x: A, y: A :: inGroup(g,x) && inGroup(g,y) ==> inGroup(g, g.compose(x,y))
     }
 
-    predicate associativeComposition<A>(g: Group<A>) {
-        forall a,b,c :: a in g.elements && b in g.elements && c in g.elements ==> g.compose(g.compose(a,b),c) == g.compose(a, g.compose(b,c))
+    lemma GroupClosedComposition<A>(g: Group<A>, a: A, b: A)
+        requires inGroup(g, a)
+        requires inGroup(g, b)
+        ensures inGroup(g, g.compose(a, b))
+
+    ghost predicate associativeComposition<A(!new)>(g: Group<A>) {
+        forall a,b,c :: inGroup(g, a) && inGroup(g, a) && inGroup(g,a) ==> g.compose(g.compose(a,b),c) == g.compose(a, g.compose(b,c))
     }
 
-    predicate commutativeComposition<A>(g: Group<A>) {
-        forall a,b :: a in g.elements && b in g.elements ==> g.compose(a,b) == g.compose(b,a)
+    lemma GroupAssociativeComposition<A>(g: Group<A>, a: A, b: A, c: A)
+        requires inGroup(g, a)
+        requires inGroup(g, b)
+        requires inGroup(g, c)
+        ensures g.compose(g.compose(a,b),c) == g.compose(a, g.compose(b,c))
+
+
+    ghost predicate commutativeComposition<A(!new)>(g: Group<A>) {
+        forall a,b :: inGroup(g, a) && inGroup(g, a) ==> g.compose(a,b) == g.compose(b,a)
     }
 
     //problematic, aka recursive trigger, it generates new patterns that match the trigger
-    predicate containsInverses<A>(g: Group<A>) {
-        forall x :: x in g.elements ==> exists xbar :: xbar in g.elements && g.compose(x,xbar) == g.identity
+    ghost predicate containsInverses<A(!new)>(g: Group<A>) {
+        forall x :: inGroup(g, x) ==> exists xbar :: inGroup(g, xbar) && g.compose(x,xbar) == g.identity
     }
+
+    lemma GroupContainsInverse<A>(g: Group<A>, x: A)
+        requires inGroup(g, x)
+        ensures inGroup(g, g.inverse(x))
+
     predicate PleaseInstantiateMe<A>(x: A) {
         true
     }
@@ -67,17 +90,25 @@ module Artin {
     //     exists xbar :: 
     //       xbar in g.elements && g.compose(x,xbar) == g.identity
     // }
-    predicate closedInverse<A>(g: Group<A>) {
-    forall x {:trigger g.inverse(x)} :: x in g.elements ==> g.inverse(x) in g.elements
+    ghost predicate closedInverse<A(!new)>(g: Group<A>) {
+        // forall x {:trigger g.inverse(x)} :: x in g.elements ==> g.inverse(x) in g.elements
+        forall x {:trigger g.inverse(x)} :: inGroup(g,x) ==> inGroup(g,g.inverse(x))
     }
 
-    predicate isInverse<A>(g: Group<A>) {
-    forall x {:trigger g.inverse(x)} :: x in g.elements ==> g.compose(x,g.inverse(x)) == g.identity && g.compose(g.inverse(x),x) == g.identity
+    ghost predicate isInverse<A(!new)>(g: Group<A>) {
+        // forall x {:trigger g.inverse(x)} :: x in g.elements ==> g.compose(x,g.inverse(x)) == g.identity && g.compose(g.inverse(x),x) == g.identity
+        forall x {:trigger g.inverse(x)} :: inGroup(g,x) ==> g.compose(x,g.inverse(x)) == g.identity && g.compose(g.inverse(x),x) == g.identity
     }
+    
+    lemma GroupInverse<A>(g: Group<A>, x: A)
+        requires inGroup(g, x)
+        ensures g.compose(x,g.inverse(x)) == g.identity && g.compose(g.inverse(x),x) == g.identity
+
 
     lemma areInverses<A>(g: Group<A>, a: A,  b: A)
         requires ValidGroup(g)
         requires a in g.elements && b in g.elements
+        requires inGroup(g,a) && inGroup(g,b)
         requires g.compose(a, b) == g.identity && g.compose(b,a) == g.identity
         ensures g.inverse(a) == b && g.inverse(b) == a
     {
@@ -88,8 +119,9 @@ module Artin {
         }
     }
 
-    predicate ValidGroup<A>(g: Group<A>) {
-        g.identity in g.elements &&
+    ghost predicate ValidGroup<A(!new)>(g: Group<A>) {
+        // g.identity in g.elements &&
+        inGroup(g, g.identity) &&
         isIdentity(g) &&
         closedComposition(g) &&
         associativeComposition(g) &&
@@ -98,7 +130,7 @@ module Artin {
         // containsInverses(g)
     }
 
-    predicate ValidSubGroup<A>(g: Group<A>, h: Group<A>) {
+    ghost predicate ValidSubGroup<A(!new)>(g: Group<A>, h: Group<A>) {
         h.elements <= g.elements &&
         g.identity in h.elements &&
         g.identity == h.identity &&
@@ -107,14 +139,14 @@ module Artin {
         // containsInverses(h)
     }
 
-    predicate AbelianGroup<A>(g: Group<A>) {
+    ghost predicate AbelianGroup<A(!new)>(g: Group<A>) {
         ValidGroup(g) && commutativeComposition(g)
     }
 
     lemma {:verify true} groupCompositionInverse<A>(g: Group<A>, a: A, b: A, abar: A, bbar: A, abbar: A)
         requires ValidGroup(g)
-        requires a in g.elements
-        requires b in g.elements
+        requires inGroup(g, a)
+        requires inGroup(g,b)
         requires g.inverse(a) == abar
         requires g.inverse(b) == bbar
         requires g.inverse(g.compose(a,b)) == abbar
@@ -132,10 +164,17 @@ module Artin {
         //     g.identity;
         // }
     }
+    /*
+function realExp(r: real, e: int): real decreases if e > 0 then e else -e {
+  if e == 0 then r
+  else if e < 0 then realExp(r/10.0, e+1)
+  else realExp(r*10.0, e-1)
+}
+    */
 
     //apow is short for abstract power
     function apow<A>(g: Group, elem: A, n: int): A
-        decreases n*n
+        decreases if n > 0 then n else -n
         ensures n == 0 ==> apow(g,elem,n) == g.identity
     {
         if n == 0 then g.identity else if n > 0 then g.compose(elem, apow(g, elem, n-1)) else if n < 0 then g.compose(g.inverse(elem), apow(g, elem, n+1)) else g.identity
@@ -155,7 +194,7 @@ module Artin {
     lemma onePower<A>(g: Group, elem: A)
         requires elem in g.elements
         requires isIdentity(g)
-        ensures apow(g, elem, 1) == elem;
+        ensures apow(g, elem, 1) == elem
     {
         calc {
             apow(g, elem, 1);
@@ -166,34 +205,48 @@ module Artin {
     }
 
     lemma oneMinusPower<A>(g: Group, elem: A)
-        requires elem in g.elements
-        requires isIdentity(g)
-        requires closedInverse(g) && isInverse(g)
-        ensures apow(g, elem, -1) == g.inverse(elem);
+        // requires elem in g.elements
+        requires inGroup(g, elem)
+        // requires isIdentity(g)
+        // requires closedInverse(g) && isInverse(g)
+        ensures apow(g, elem, -1) == g.inverse(elem)
     {
+        GroupContainsInverse(g, elem);
+        calc {
+            apow(g, elem, -1);
+            g.compose(g.inverse(elem), apow(g, elem, 0));
+            g.compose(g.inverse(elem), g.identity);
+            == {GroupIdentity(g, g.inverse(elem));}
+            g.inverse(elem);
+        }
     }
 
     lemma {:verify true} apowClosed<A>(g: Group, elem: A, n: int)
-        requires elem in g.elements
-        requires g.identity in g.elements
+        // requires elem in g.elements
+        // requires g.identity in g.elements
+        requires inGroup(g, elem)
+        requires inGroup(g, g.identity)
         // requires isIdentity(g)
-        requires closedComposition(g)
-        requires closedInverse(g)
+        // requires closedComposition(g)
+        // requires closedInverse(g)
         // requires isInverse(g)
         // requires n >= 0
         decreases n*n
-        ensures apow(g, elem, n) in g.elements
+        ensures inGroup(g, apow(g, elem, n))
     {
         if n == 0 {
             assert apow(g, elem, 0) in g.elements;
         } else if n > 0 {
             apowPos(g, elem, n);
-            // apowClosed(g, elem, n-1);
+            apowClosed(g, elem, n-1);
+            GroupClosedComposition(g, elem, apow(g, elem, n-1));
         }else {
             apowNegative(g,elem, n);
             apowClosed(g, elem, n+1);
             assert apow(g, elem, n+1) in g.elements;
             assert elem in g.elements;
+            GroupContainsInverse(g, elem);
+            GroupClosedComposition(g, g.inverse(elem), apow(g, elem, n+1));
             // calc {
             //     apow(g, elem, n);
             //     g.compose(g.inverse(elem), )
@@ -202,12 +255,18 @@ module Artin {
         }
 }
 
+    predicate inGroup<A>(g: Group, elem: A) {
+        elem in g.elements
+    }
+
     lemma {:verify true} allApowClosed<A>(g: Group, elem: A) 
-        requires closedComposition(g)
-        requires closedInverse(g)
-        requires g.identity in g.elements
-        requires elem in g.elements
-        ensures forall x: int :: apow(g, elem, x) in g.elements
+        // requires closedComposition(g)
+        // requires closedInverse(g)
+        // requires g.identity in g.elements
+        // requires elem in g.elements
+        requires inGroup(g, g.identity)
+        requires inGroup(g, elem)
+        ensures forall x: int :: inGroup(g, apow(g, elem, x))
     {
         forall x: int | true 
         {
@@ -216,31 +275,53 @@ module Artin {
     }
 
     // method {:verify true} apowSubtract<A>(g: Group<A>, elem: A, n: int)
-    lemma {:verify true} {:induction false} apowSubtract<A>(g: Group<A>, elem: A, n: int)
-        requires ValidGroup(g)
-        requires elem in g.elements
+    lemma {:verify } {:induction false} apowSubtract<A(!new)>(g: Group<A>, elem: A, n: int)
+        // requires ValidGroup(g)
+        // requires closedComposition(g)
+        // requires closedInverse(g)
+        // requires associativeComposition(g)
+        // requires isIdentity(g)
+        // requires isInverse(g)
+        // requires g.identity in g.elements
+        // requires elem in g.elements
+        requires inGroup(g, g.identity)
+        requires inGroup(g, elem)
         requires n >= 0
         // ensures g.compose(apow(g, elem, n), apow(g, elem, -1)) == apow(g, elem, n-1)
         ensures g.compose(apow(g, elem, -1), apow(g, elem, n)) == apow(g, elem, n-1)
     {
         allApowClosed(g, elem);
+        assert inGroup(g, apow(g, elem, -1));
+        assert inGroup(g, apow(g, elem, n));
+        assert inGroup(g, apow(g, elem, n-1));
+        assert inGroup(g, g.identity);
         if n > 0 {
             calc {
                 g.compose(apow(g, elem, -1), apow(g, elem, n));
-                // == {apowPos(g,elem, n);}
+                == {apowPos(g,elem, n);}
                 g.compose(apow(g, elem, -1), g.compose(elem, apow(g, elem, n-1)));
+                == {GroupAssociativeComposition(g,apow(g, elem, -1), elem, apow(g, elem, n-1));}
                 g.compose(g.compose(apow(g, elem, -1), elem), apow(g, elem, n-1));
+                == {oneMinusPower(g, elem);}
                 g.compose(g.compose(g.inverse(elem), elem), apow(g, elem, n-1));
+                == {GroupInverse(g, elem);}
                 g.compose(g.identity, apow(g, elem, n-1));
+                == {GroupIdentity(g, apow(g, elem, n-1));}
                 apow(g, elem, n-1);
             }
         }else if n == 0 {
+            calc {
+                g.compose(apow(g, elem, -1), apow(g, elem, 0));
+                g.compose(apow(g, elem, -1), g.identity);
+                == {GroupIdentity(g, apow(g, elem, -1));}
+                apow(g, elem, -1);
+            }
         }else{
             assert n < 0;
             assert (n-1)+1 == n;
             calc {
                 g.compose(apow(g, elem, -1), apow(g, elem, n));
-                g.compose(apow(g, elem, -1), apow(g, elem, n));
+                == {oneMinusPower(g, elem);}
                 g.compose(g.inverse(elem), apow(g, elem, n));
                 apow(g, elem, n-1);
             }
@@ -254,13 +335,16 @@ module Artin {
         ensures g.compose(apow(g, elem, -n), apow(g, elem, -k)) == apow(g, elem, -n-k)
 
     lemma {:verify true} apowAddition<A>(g: Group<A>, elem: A, n: nat, k: nat)
-        requires elem in g.elements
+        // requires elem in g.elements
+        // requires g.identity in g.elements
+        requires inGroup(g, elem)
+        requires inGroup(g, g.identity)
         // requires ValidGroup(g)
-        requires closedComposition(g)
-        requires closedInverse(g)
-        requires g.identity in g.elements
-        requires isIdentity(g);
-        requires associativeComposition(g)
+        // requires closedComposition(g)
+        // requires closedInverse(g)
+        // requires inGroup(g, g.identity)
+        // requires isIdentity(g)
+        // requires associativeComposition(g)
         ensures g.compose(apow(g, elem, n), apow(g, elem, k)) == apow(g, elem, n+k)
     {
         allApowClosed(g, elem);
@@ -270,15 +354,18 @@ module Artin {
                 apow(g, elem, n+k);
                 apow(g, elem, n);
             }
+            GroupIdentity(g, apow(g, elem, n));
             assert g.compose(apow(g, elem, n), g.identity) == apow(g, elem, n+k);
         }else if n == 0 {
             assert apow(g, elem, n) == g.identity;
+            GroupIdentity(g, apow(g, elem, k));
             assert g.compose(g.identity, apow(g, elem, k)) == apow(g, elem, n+k);
         }else if n > 0 {
             apowPos(g,elem, n);
             calc {
                 g.compose(apow(g, elem, n), apow(g, elem, k));
                 g.compose(g.compose(elem, apow(g, elem, n-1)), apow(g, elem, k));
+                == {GroupAssociativeComposition(g, elem, apow(g, elem, n-1), apow(g, elem, k));}
                 g.compose(elem, g.compose(apow(g, elem, n-1), apow(g, elem, k)));
                 == {apowAddition(g,elem, n-1,k);}
                 g.compose(elem, apow(g, elem, n-1+k));
@@ -289,7 +376,7 @@ module Artin {
 
     lemma apowInverse<A>(g: Group<A>, elem: A, n: int)
         requires elem in g.elements
-        requires n >= 0;
+        requires n >= 0
         requires ValidGroup(g)
         // ensures g.inverse(apow(g,elem, n)) == apow(g, elem, -n)
     {
@@ -319,7 +406,7 @@ module Artin {
         // requires closedComposition(g)
         // requires closedInverse(g)
         requires g.identity in g.elements
-        requires isIdentity(g);
+        requires isIdentity(g)
         requires associativeComposition(g)
         // ensures g.compose(apow(g, elem, n), apow(g, elem, k)) == apow(g, elem, n+k)
     {
@@ -377,18 +464,18 @@ module Artin {
     }
 
     lemma positiveNumbersArePositive(k: nat, s: nat)
-        requires k >= 0;
-        requires s >= 0;
+        requires k >= 0
+        requires s >= 0
         ensures Math.prod(k , s) >= 0
     {
         reveal Math.prod();
     }
 
     lemma positiveNumbersAreStilPositive(k: nat, s: nat, x: nat, y: nat)
-        requires k >= 0;
-        requires s >= 0;
-        requires x >= 0;
-        requires y >= 0;
+        requires k >= 0
+        requires s >= 0
+        requires x >= 0
+        requires y >= 0
         ensures Math.prod(k , s) + Math.prod(x,y) >= 0
     {
         positiveNumbersArePositive(k,s);
@@ -424,19 +511,23 @@ module Artin {
 
     }
 
-    lemma something<A>(g: Group<A>, elem: A, k: nat, s: nat)
+    lemma {:verify }  something<A>(g: Group<A>, elem: A, k: nat, s: nat)
         requires elem in g.elements
         // requires ValidGroup(g)
-        requires closedComposition(g)
-        requires closedInverse(g)
+        // requires closedComposition(g)
+        // requires closedInverse(g)
         requires g.identity in g.elements
-        requires isIdentity(g);
-        requires associativeComposition(g)
+        // requires isIdentity(g)
+        // requires associativeComposition(g)
         requires s >= 1
-        ensures g.compose(apow(g, elem, k), apow(g, elem, k*(s-1))) == apow(g, elem, k + k*(s-1))
+        // ensures g.compose(apow(g, elem, k), apow(g, elem, k*(s-1))) == apow(g, elem, k + k*(s-1))
+         ensures g.compose(apow(g, elem, k), apow(g, elem, Math.prod(k,(s-1)))) == apow(g, elem, k+Math.prod(k,(s-1)))
     {
-        apowAddition(g, elem, k, k*(s-1));
+        reveal Math.prod();
+        assert Math.prod(k, (s-1)) >= 0;
+        apowAddition(g, elem, k, Math.prod(k,(s-1)));
     }
+
     lemma something2<A>(g: Group<A>, elem: A, k: nat, s: nat)
         requires s >= 1
         ensures apow(g, elem, k*s) == apow(g, elem, k + k*(s-1))
@@ -444,15 +535,15 @@ module Artin {
         // assert k+k*(s-1) == k * s;
     }
 
-    lemma {:verify }  apowExponentNat<A>(g: Group<A>, elem: A, k: nat, s: nat)
+    lemma {:verify false}  apowExponentNat<A>(g: Group<A>, elem: A, k: nat, s: nat)
         requires elem in g.elements
         // requires ValidGroup(g)
         requires closedComposition(g)
         requires closedInverse(g)
         requires g.identity in g.elements
-        requires isIdentity(g);
+        requires isIdentity(g)
         requires associativeComposition(g)
-        ensures apow(g, apow(g, elem, k), s) == apow(g, elem, k*s);
+        ensures apow(g, apow(g, elem, k), s) == apow(g, elem, k*s)
     {
         if s == 0 {
             // assert k * s == 0;
@@ -474,16 +565,17 @@ module Artin {
         }
     }
 
-    lemma {:verify false}  apowExponent<A>(g: Group<A>, elem: A, k: nat, s: nat) //works but is slow
-        requires elem in g.elements
+    lemma {:verify }  apowExponent<A>(g: Group<A>, elem: A, k: nat, s: nat)
+        requires inGroup(g, elem)
+        requires inGroup(g, g.identity)
         // requires ValidGroup(g)
-        requires closedComposition(g)
-        requires closedInverse(g)
-        requires g.identity in g.elements
-        requires isIdentity(g);
-        requires associativeComposition(g)
+        // requires closedComposition(g)
+        // requires closedInverse(g)
+        // requires inGroup(g, g.identity)
+        // requires isIdentity(g)
+        // requires associativeComposition(g)
         // ensures apow(g, apow(g, elem, k), s) == apow(g, elem, k*s);
-        ensures apow(g, apow(g, elem, k), s) == apow(g, elem, Math.prod(k,s));
+        ensures apow(g, apow(g, elem, k), s) == apow(g, elem, Math.prod(k,s))
     {
         allApowClosed(g,elem);
         allApowClosed(g,apow(g,elem, k));
@@ -498,7 +590,7 @@ module Artin {
             positiveNumbersArePositive(k, sub(s,1));
             positiveNumbersAreStilPositive(k,1,k,sub(s,1));
             assert Math.prod(k,1)+Math.prod(k,sub(s,1)) >= 0;
-            // assume apow(g, apow(g, elem, k), sub(s,1)) == apow(g, elem, Math.prod(k,sub(s,1)));
+            // // assume apow(g, apow(g, elem, k), sub(s,1)) == apow(g, elem, Math.prod(k,sub(s,1)));
             assert k + Math.prod(k,sub(s,1)) >=0;
             calc {
                 apow(g, apow(g, elem, k), s);
@@ -554,7 +646,7 @@ module Artin {
             // }
      */
 
-    predicate CyclicGroupGeneratedBy<A(!new)>(g: Group, elem: A)
+    ghost predicate CyclicGroupGeneratedBy<A(!new)>(g: Group, elem: A)
         requires elem in g.elements
     {
         exists n :: n == |g.elements| &&
@@ -564,13 +656,13 @@ module Artin {
             forall x :: x in g.elements && exists n :: apow(g, elem, n) == x
     }
 
-    predicate isIsomorphism<A,B>(g: Group<A>, g': Group<B>, phi: A -> B)
+    ghost predicate isIsomorphism<A,B>(g: Group<A>, g': Group<B>, phi: A -> B)
         requires ValidGroup(g)
         requires ValidGroup(g')
     {
         phi(g.identity) == g'.identity &&
-        forall x :: x in g.elements ==> phi(x) in g'.elements &&
-        forall x,y :: x in g.elements && y in g.elements ==> phi(g.compose(x,y)) == g'.compose(phi(x), phi(y))
+        forall x :: x in g.elements ==> (phi(x) in g'.elements &&
+        forall x,y :: x in g.elements && y in g.elements ==> phi(g.compose(x,y)) == g'.compose(phi(x), phi(y)))
     }
 
     lemma Artin2_3_b<A,B>(g: Group<A>, g': Group<B>, phi: A -> B, x: A, y: A) 
